Prove paxos crash recovery

external/Goose/github_com/mit_pdos/tulip/paxos.v
@@ -853,76 +853,56 @@ Definition resume: val :=
     let: "terml" := ref (zero_val uint64T) in
     let: "lsnc" := ref (zero_val uint64T) in
     let: "log" := ref_to (slice.T stringT) (NewSlice stringT #0) in
-    let: "kind" := ref (zero_val uint64T) in
-    let: "term" := ref (zero_val uint64T) in
-    let: "lsn" := ref (zero_val uint64T) in
-    let: "ents" := ref (zero_val (slice.T stringT)) in
     let: "data" := ref_to (slice.T byteT) (grove_ffi.FileRead "fname") in
     Skip;;
     (for: (λ: <>, #0 < (slice.len (![slice.T byteT] "data"))); (λ: <>, Skip) := λ: <>,
-      let: ("0_ret", "1_ret") := marshal.ReadInt (![slice.T byteT] "data") in
-      "kind" <-[uint64T] "0_ret";;
-      "data" <-[slice.T byteT] "1_ret";;
-      (if: (![uint64T] "kind") = CMD_EXTEND
+      let: ("kind", "bs") := marshal.ReadInt (![slice.T byteT] "data") in
+      (if: "kind" = CMD_EXTEND
       then
-        let: ("0_ret", "1_ret") := util.DecodeStrings (![slice.T byteT] "data") in
-        "ents" <-[slice.T stringT] "0_ret";;
-        "data" <-[slice.T byteT] "1_ret";;
-        "log" <-[slice.T stringT] (SliceAppendSlice stringT (![slice.T stringT] "log") (![slice.T stringT] "ents"));;
+        let: ("ents", "bs1") := util.DecodeStrings "bs" in
+        "data" <-[slice.T byteT] "bs1";;
+        "log" <-[slice.T stringT] (SliceAppendSlice stringT (![slice.T stringT] "log") "ents");;
         Continue
       else
-        (if: (![uint64T] "kind") = CMD_APPEND
+        (if: "kind" = CMD_APPEND
         then
-          "ents" <-[slice.T stringT] (NewSlice stringT #1);;
-          let: "ent" := ref (zero_val stringT) in
-          let: ("0_ret", "1_ret") := util.DecodeString (![slice.T byteT] "data") in
-          "ent" <-[stringT] "0_ret";;
-          "data" <-[slice.T byteT] "1_ret";;
-          "log" <-[slice.T stringT] (SliceAppend stringT (![slice.T stringT] "log") (![stringT] "ent"));;
+          let: ("ent", "bs1") := util.DecodeString "bs" in
+          "data" <-[slice.T byteT] "bs1";;
+          "log" <-[slice.T stringT] (SliceAppend stringT (![slice.T stringT] "log") "ent");;
           Continue
         else
-          (if: (![uint64T] "kind") = CMD_PREPARE
+          (if: "kind" = CMD_PREPARE
           then
-            let: ("0_ret", "1_ret") := marshal.ReadInt (![slice.T byteT] "data") in
-            "term" <-[uint64T] "0_ret";;
-            "data" <-[slice.T byteT] "1_ret";;
-            "termc" <-[uint64T] (![uint64T] "term");;
+            let: ("term", "bs1") := marshal.ReadInt "bs" in
+            "data" <-[slice.T byteT] "bs1";;
+            "termc" <-[uint64T] "term";;
             Continue
           else
-            (if: (![uint64T] "kind") = CMD_ADVANCE
+            (if: "kind" = CMD_ADVANCE
             then
-              let: ("0_ret", "1_ret") := marshal.ReadInt (![slice.T byteT] "data") in
-              "term" <-[uint64T] "0_ret";;
-              "data" <-[slice.T byteT] "1_ret";;
-              let: ("0_ret", "1_ret") := marshal.ReadInt (![slice.T byteT] "data") in
-              "lsn" <-[uint64T] "0_ret";;
-              "data" <-[slice.T byteT] "1_ret";;
-              let: ("0_ret", "1_ret") := util.DecodeStrings (![slice.T byteT] "data") in
-              "ents" <-[slice.T stringT] "0_ret";;
-              "data" <-[slice.T byteT] "1_ret";;
-              "terml" <-[uint64T] (![uint64T] "term");;
-              "log" <-[slice.T stringT] (SliceTake (![slice.T stringT] "log") (![uint64T] "lsn"));;
-              "log" <-[slice.T stringT] (SliceAppendSlice stringT (![slice.T stringT] "log") (![slice.T stringT] "ents"));;
+              let: ("term", "bs1") := marshal.ReadInt "bs" in
+              let: ("lsn", "bs2") := marshal.ReadInt "bs1" in
+              let: ("ents", "bs3") := util.DecodeStrings "bs2" in
+              "data" <-[slice.T byteT] "bs3";;
+              "terml" <-[uint64T] "term";;
+              "log" <-[slice.T stringT] (SliceTake (![slice.T stringT] "log") "lsn");;
+              "log" <-[slice.T stringT] (SliceAppendSlice stringT (![slice.T stringT] "log") "ents");;
               Continue
             else
-              (if: (![uint64T] "kind") = CMD_ACCEPT
+              (if: "kind" = CMD_ACCEPT
               then
-                let: ("0_ret", "1_ret") := marshal.ReadInt (![slice.T byteT] "data") in
-                "lsn" <-[uint64T] "0_ret";;
-                "data" <-[slice.T byteT] "1_ret";;
-                let: ("0_ret", "1_ret") := util.DecodeStrings (![slice.T byteT] "data") in
-                "ents" <-[slice.T stringT] "0_ret";;
-                "data" <-[slice.T byteT] "1_ret";;
-                "log" <-[slice.T stringT] (SliceTake (![slice.T stringT] "log") (![uint64T] "lsn"));;
-                "log" <-[slice.T stringT] (SliceAppendSlice stringT (![slice.T stringT] "log") (![slice.T stringT] "ents"));;
+                let: ("lsn", "bs1") := marshal.ReadInt "bs" in
+                let: ("ents", "bs2") := util.DecodeStrings "bs1" in
+                "data" <-[slice.T byteT] "bs2";;
+                "log" <-[slice.T stringT] (SliceTake (![slice.T stringT] "log") "lsn");;
+                "log" <-[slice.T stringT] (SliceAppendSlice stringT (![slice.T stringT] "log") "ents");;
                 Continue
               else
-                (if: (![uint64T] "kind") = CMD_EXPAND
+                (if: "kind" = CMD_EXPAND
                 then
-                  let: ("0_ret", "1_ret") := marshal.ReadInt (![slice.T byteT] "data") in
-                  "lsn" <-[uint64T] "0_ret";;
-                  "data" <-[slice.T byteT] "1_ret";;
-                  "lsnc" <-[uint64T] (![uint64T] "lsn");;
+                  let: ("lsn", "bs1") := marshal.ReadInt "bs" in
+                  "data" <-[slice.T byteT] "bs1";;
+                  "lsnc" <-[uint64T] "lsn";;
                   Continue
                 else Continue)))))));;
     (![uint64T] "termc", ![uint64T] "terml", ![uint64T] "lsnc", ![slice.T stringT] "log").
