src/program_proof/tulip/encode.v
@@ -1,55 +1,33 @@
 From Perennial.program_proof Require Import grove_prelude.
 From Perennial.program_proof.tulip Require Import base.
+From Perennial.program_proof.rsm Require Import serialize.
 
 Definition encode_string (x : byte_string) : list u8 :=
   u64_le (U64 (length x)) ++ x.
 
-Definition encode_strings_step (bs : list u8) (x : byte_string) : list u8 :=
-  bs ++ encode_string x.
-
 Definition encode_strings_xlen (xs : list byte_string) : list u8 :=
-  foldl encode_strings_step [] xs.
+  serialize encode_string xs.
 
 Definition encode_strings (xs : list byte_string) : list u8 :=
   u64_le (U64 (length xs)) ++ encode_strings_xlen xs.
 
 Lemma encode_strings_xlen_snoc xs x :
   encode_strings_xlen (xs ++ [x]) = encode_strings_xlen xs ++ encode_string x.
-Proof.
-  by rewrite /encode_strings_xlen foldl_snoc /encode_strings_step.
-Qed.
-
-Lemma foldl_encode_strings_step_app (bs : list u8) (xs : list byte_string) :
-  foldl encode_strings_step bs xs = bs ++ foldl encode_strings_step [] xs.
-Proof.
-  generalize dependent bs.
-  induction xs as [| x xs IH]; intros bs.
-  { by rewrite /= app_nil_r. }
-  rewrite /= (IH (encode_strings_step bs x)) (IH (encode_strings_step [] x)).
-  rewrite {1 3}/encode_strings_step.
-  by rewrite app_nil_l app_assoc.
-Qed.
+Proof. by rewrite /encode_strings_xlen serialize_snoc. Qed.
 
 Lemma encode_strings_xlen_cons xs x :
   encode_strings_xlen (x :: xs) = encode_string x ++ encode_strings_xlen xs.
-Proof.
-  rewrite /encode_strings_xlen /= foldl_encode_strings_step_app.
-  by rewrite {1}/encode_strings_step app_nil_l.
-Qed.
+Proof. by rewrite /encode_strings_xlen serialize_cons. Qed.
 
 Lemma encode_strings_xlen_length_inv xs n :
   (length (encode_strings_xlen xs) ≤ n)%nat ->
   (length xs ≤ n)%nat.
 Proof.
-  generalize dependent n.
-  induction xs as [| x xs IH]; intros n; first done.
-  rewrite encode_strings_xlen_cons length_app /=.
-  assert (length (encode_string x) ≠ O).
-  { by destruct (nil_or_length_pos (encode_string x)). }
+  rewrite /encode_strings_xlen.
   intros Hlen.
-  assert (Hlenxs : (length xs ≤ pred n)%nat).
-  { apply IH. lia. }
-  lia.
+  apply (serialize_length_inv encode_string).
+  { intros x. by destruct (nil_or_length_pos (encode_string x)). }
+  done.
 Qed.
 
 Lemma encode_strings_length_inv xs n :
@@ -71,52 +49,29 @@ Definition encode_dbval (x : dbval) : list u8 :=
 Definition encode_dbmod (x : dbmod) : list u8 :=
   encode_string x.1 ++ encode_dbval x.2.
 
-Definition encode_dbmods_step (bs : list u8) (x : dbmod) : list u8 :=
-  bs ++ encode_dbmod x.
-
 Definition encode_dbmods_xlen (xs : list dbmod) : list u8 :=
-  foldl encode_dbmods_step [] xs.
+  serialize encode_dbmod xs.
 
 Definition encode_dbmods (xs : list dbmod) : list u8 :=
   u64_le (U64 (length xs)) ++ encode_dbmods_xlen xs.
 
 Lemma encode_dbmods_xlen_snoc xs x :
   encode_dbmods_xlen (xs ++ [x]) = encode_dbmods_xlen xs ++ encode_dbmod x.
-Proof.
-  by rewrite /encode_dbmods_xlen foldl_snoc /encode_dbmods_step.
-Qed.
-
-Lemma foldl_encode_dbmods_step_app (bs : list u8) (xs : list dbmod) :
-  foldl encode_dbmods_step bs xs = bs ++ foldl encode_dbmods_step [] xs.
-Proof.
-  generalize dependent bs.
-  induction xs as [| x xs IH]; intros bs.
-  { by rewrite /= app_nil_r. }
-  rewrite /= (IH (encode_dbmods_step bs x)) (IH (encode_dbmods_step [] x)).
-  rewrite {1 3}/encode_dbmods_step.
-  by rewrite app_nil_l app_assoc.
-Qed.
+Proof. by rewrite /encode_dbmods_xlen serialize_snoc. Qed.
 
 Lemma encode_dbmods_xlen_cons xs x :
   encode_dbmods_xlen (x :: xs) = encode_dbmod x ++ encode_dbmods_xlen xs.
-Proof.
-  rewrite /encode_dbmods_xlen /= foldl_encode_dbmods_step_app.
-  by rewrite {1}/encode_dbmods_step app_nil_l.
-Qed.
+Proof. by rewrite /encode_dbmods_xlen serialize_cons. Qed.
 
 Lemma encode_dbmods_xlen_length_inv xs n :
   (length (encode_dbmods_xlen xs) ≤ n)%nat ->
   (length xs ≤ n)%nat.
 Proof.
-  generalize dependent n.
-  induction xs as [| x xs IH]; intros n; first done.
-  rewrite encode_dbmods_xlen_cons length_app /=.
-  assert (length (encode_dbmod x) ≠ O).
-  { by destruct x as [[] []]. }
+  rewrite /encode_dbmods_xlen.
   intros Hlen.
-  assert (Hlenxs : (length xs ≤ pred n)%nat).
-  { apply IH. lia. }
-  lia.
+  apply (serialize_length_inv encode_dbmod).
+  { intros x. by destruct (nil_or_length_pos (encode_dbmod x)). }
+  done.
 Qed.
 
 Lemma encode_dbmods_length_inv xs n :
