src/program_proof/tulip/paxos/program/paxos_commit.v
@@ -90,9 +90,19 @@ Section commit.
       iApply ncfupd_mask_intro; first solve_ndisj.
       iIntros "Hmask".
       iDestruct (node_wal_fname_agree with "Hfnameme Hwalfname") as %->.
-      iFrame "Hfile".
-      iExists wal.
-      iIntros (bs') "[Hfile %Hbs']".
+      iFrame "Hfile %".
+      iIntros (bs' failed) "Hfile".
+      destruct failed.
+      { (* Case: Write failed. Close the invariant without any updates. *)
+        iMod "Hmask" as "_".
+        iDestruct ("HinvfileO" with "[Hfile Hwalfile]") as "HinvfileO".
+        { iFrame "∗ # %". }
+        iMod ("HinvfileC" with "HinvfileO") as "_".
+        iMod ("HinvC" with "HinvO") as "_".
+        by iIntros "!> %Hcontra".
+      }
+      (* Case: Write succeeded. *)
+      iDestruct "Hfile" as "[Hfile %Hbs']".
       iMod (paxos_inv_expand (length log) with "[Hsafe'] Hwalfile Hterml Hlsnc Hlogn HinvO")
         as "(Hwalfile & Hterml & Hlsnc & Hlogn & HinvO)".
       { apply Hnidme. }
@@ -101,7 +111,12 @@ Section commit.
       { by rewrite Hszlog. }
       rewrite -Hszlog in Hbs'.
       iDestruct ("HinvfileO" with "[Hfile Hwalfile]") as "HinvfileO".
-      { iFrame "∗ # %". }
+      { iFrame "∗ # %".
+        iPureIntro.
+        apply Forall_app_2; first apply Hvdwal.
+        rewrite Forall_singleton /=.
+        word.
+      }
       iMod "Hmask" as "_".
       iMod ("HinvfileC" with "HinvfileO") as "_".
       iMod ("HinvC" with "HinvO") as "_".
@@ -139,9 +154,19 @@ Section commit.
     iApply ncfupd_mask_intro; first solve_ndisj.
     iIntros "Hmask".
     iDestruct (node_wal_fname_agree with "Hfnameme Hwalfname") as %->.
-    iFrame "Hfile".
-    iExists wal.
-    iIntros (bs') "[Hfile %Hbs']".
+    iFrame "Hfile %".
+    iIntros (bs' failed) "Hfile".
+    destruct failed.
+    { (* Case: Write failed. Close the invariant without any updates. *)
+      iMod "Hmask" as "_".
+      iDestruct ("HinvfileO" with "[Hfile Hwalfile]") as "HinvfileO".
+      { iFrame "∗ # %". }
+      iMod ("HinvfileC" with "HinvfileO") as "_".
+      iMod ("HinvC" with "HinvO") as "_".
+      by iIntros "!> %Hcontra".
+    }
+    (* Case: Write succeeded. *)
+    iDestruct "Hfile" as "[Hfile %Hbs']".
     assert (Hprefix : prefix logc log).
     { destruct Horprefix as [Hprefix | ?]; last done.
       rewrite (prefix_length_eq _ _ Hprefix); first done.
@@ -156,7 +181,12 @@ Section commit.
     { clear -Hgtlsnc. lia. }
     { rewrite Hszlog. clear -Hlelog. lia. }
     iDestruct ("HinvfileO" with "[Hfile Hwalfile]") as "HinvfileO".
-    { iFrame "∗ # %". }
+    { iFrame "∗ # %".
+      iPureIntro.
+      apply Forall_app_2; first apply Hvdwal.
+      rewrite Forall_singleton /=.
+      word.
+    }
     iMod "Hmask" as "_".
     iMod ("HinvfileC" with "HinvfileO") as "_".
     iMod ("HinvC" with "HinvO") as "_".
