src/program_proof/tulip/paxos/program/paxos_stepdown.v
@@ -53,15 +53,30 @@ Section stepdown.
     iApply ncfupd_mask_intro; first solve_ndisj.
     iIntros "Hmask".
     iDestruct (node_wal_fname_agree with "Hfnameme Hwalfname") as %->.
-    iFrame "Hfile".
-    iExists wal.
-    iIntros (bs') "[Hfile %Hbs']".
+    iFrame "Hfile %".
+    iIntros (bs' failed) "Hfile".
+    destruct failed.
+    { (* Case: Write failed. Close the invariant without any updates. *)
+      iMod "Hmask" as "_".
+      iDestruct ("HinvfileO" with "[Hfile Hwalfile]") as "HinvfileO".
+      { iFrame "∗ # %". }
+      iMod ("HinvfileC" with "HinvfileO") as "_".
+      iMod ("HinvC" with "HinvO") as "_".
+      by iIntros "!> %Hcontra".
+    }
+    (* Case: Write succeeded. *)
+    iDestruct "Hfile" as "[Hfile %Hbs']".
     iMod (paxos_inv_prepare (uint.nat term) with "Hwalfile Htermc Hterml Hlogn HinvO")
       as "(Hwalfile & Htermc & Hterml & Hlogn & HinvO & Hlsnp & #Hpromise)".
     { apply Hnidme. }
     { clear -Hlt Hne. apply u64_val_ne in Hne. word. }
     iDestruct ("HinvfileO" with "[Hfile Hwalfile]") as "HinvfileO".
-    { iFrame "∗ # %". }
+    { iFrame "∗ # %".
+      iPureIntro.
+      apply Forall_app_2; first apply Hvdwal.
+      rewrite Forall_singleton /=.
+      word.
+    }
     iMod "Hmask" as "_".
     (* iMod ("Hclose_termc" with "Htermc") as "Htermc". *)
     iMod ("HinvfileC" with "HinvfileO") as "_".
