src/program_proof/tulip/paxos/program/resume.v
@@ -1,10 +1,69 @@
+From Perennial.program_proof.rsm.pure Require Import serialize.
+From Perennial.program_proof Require Import marshal_stateless_proof.
+From Perennial.program_proof.tulip.program.util Require Import
+  decode_string decode_strings.
 From Perennial.program_proof.tulip.paxos Require Import prelude.
 From Goose.github_com.mit_pdos.tulip Require Import paxos.
+
+Opaque u64_le.
+
+(* Copy pasted from grove_ffi_typed.v *)
+Ltac inv_undefined :=
+  match goal with
+  | [ H: relation.denote (match ?e with | _ => _ end) _ _ _ |- _ ] =>
+    destruct e; try (apply suchThat_false in H; contradiction)
+  end.
+Local Ltac solve_atomic :=
+  apply strongly_atomic_atomic, ectx_language_atomic;
+  [ apply heap_base_atomic; cbn [relation.denote base_trans]; intros * H;
+    repeat inv_undefined;
+    try solve [ apply atomically_is_val in H; auto ]
+    |apply ectxi_language_sub_redexes_are_values; intros [] **; naive_solver].
+Local Ltac solve_atomic2 :=
+  solve_atomic;
+  (* TODO(Joe): Cleanup *)
+  repeat match goal with
+    | [ H: relation.denote _ ?s1 ?s2 ?v |- _ ] => inversion_clear H
+    | _ => progress monad_inv
+    | _ => case_match
+    end; eauto.
 
 Section resume.
   Context `{!heapGS Σ, !paxos_ghostG Σ}.
 
-  Theorem wp_resume (fname : byte_string) (nidme termc terml lsnc : u64) (log : list byte_string) γ :
+  Lemma paxos_recoverable_from_wal
+    (nidme : u64) (termc terml lsnc : nat) (logn : list byte_string) (wal : list pxcmd)
+    nids γ :
+    nidme ∈ nids ->
+    own_current_term_half γ nidme termc -∗
+    own_ledger_term_half γ nidme terml -∗
+    own_committed_lsn_half γ nidme lsnc -∗
+    own_node_ledger_half γ nidme logn -∗
+    own_node_wal_half γ nidme wal -∗
+    paxos_inv γ nids -∗
+    ⌜execute_paxos_cmds wal = PaxosState termc terml lsnc logn⌝.
+  Proof.
+    iIntros (Hnidme) "HtermcX HtermlX HlsncX HlognX HwalX Hinv".
+    iNamed "Hinv".
+    rewrite -Hdomtermlm elem_of_dom in Hnidme.
+    destruct Hnidme as [terml0 Hlookup].
+    iDestruct (big_sepM_lookup with "Hnodes") as "Hnode".
+    { apply Hlookup. }
+    iNamed "Hnode".
+    iDestruct (current_term_agree with "HtermcX Htermc") as %->.
+    iDestruct (ledger_term_agree with "HtermlX Hterml") as %->.
+    iDestruct (committed_lsn_agree with "HlsncX Hlsnc") as %->.
+    iDestruct (node_ledger_agree with "HlognX Hlogn") as %->.
+    by iDestruct (node_wal_agree with "HwalX Hwalnode") as %->.
+  Qed.
+
+  Theorem wp_resume
+    (fname : byte_string) (nidme termc terml lsnc : u64) (log : list byte_string)
+    nids γ :
+    nidme ∈ nids ->
+    is_node_wal_fname γ nidme fname -∗
+    know_paxos_inv γ nids -∗
+    know_paxos_file_inv γ nids -∗
     {{{ own_current_term_half γ nidme (uint.nat termc) ∗
         own_ledger_term_half γ nidme (uint.nat terml) ∗
         own_committed_lsn_half γ nidme (uint.nat lsnc) ∗
@@ -19,63 +78,393 @@ Section resume.
         own_slice logP stringT (DfracOwn 1) log
     }}}.
   Proof.
+    iIntros (Hnidme) "#Hfname #Hinv #Hinvfile".
+    iIntros (Φ) "!> (Htermc & Hterml & Hlsnc & Hlog) HΦ".
+    wp_rec.
+
     (*@ func resume(fname string) (uint64, uint64, uint64, []string) {          @*)
     (*@     var termc uint64                                                    @*)
     (*@     var terml uint64                                                    @*)
     (*@     var lsnc  uint64                                                    @*)
     (*@     var log = make([]string, 0)                                         @*)
     (*@                                                                         @*)
-    (*@     var kind uint64                                                     @*)
-    (*@     var term uint64                                                     @*)
-    (*@     var lsn  uint64                                                     @*)
-    (*@     var ents []string                                                   @*)
-    (*@                                                                         @*)
+    wp_apply wp_ref_of_zero; first done.
+    iIntros (termcP) "HtermcP".
+    wp_apply wp_ref_of_zero; first done.
+    iIntros (termlP) "HtermlP".
+    wp_apply wp_ref_of_zero; first done.
+    iIntros (lsncP) "HlsncP".
+    wp_apply wp_NewSlice.
+    iIntros (logP) "HlogP".
+    rewrite uint_nat_W64_0 /=.
+    wp_apply wp_ref_to; first done.
+    iIntros (logPP) "HlogPP".
+
     (*@     var data = grove_ffi.FileRead(fname)                                @*)
     (*@                                                                         @*)
+    wp_pures.
+    wp_rec. wp_pures.
+    wp_bind (ExternalOp _ _).
+    (* Open the file invariant to obtain (1) the file points-to, (2) encoding
+    relation between the file content and the WAL log. *)
+    iInv "Hinvfile" as "> HinvfileO" "HinvfileC".
+    { solve_atomic2. }
+    iDestruct (big_sepS_elem_of_acc with "HinvfileO") as "[Hinvnode HinvnodeC]".
+    { apply Hnidme. }
+    iNamed "Hinvnode".
+    iDestruct (node_wal_fname_agree with "Hfname Hwalfname") as %->.
+    (* Open the core invariant to obtain (1) the durable resources (e.g.,
+    [own_current_term_half]), (2) the recovery relation between the WAL log and
+    the durable resources. *)
+    iInv "Hinv" as "> HinvO" "HinvC".
+    { solve_atomic2. }
+    iDestruct (paxos_recoverable_from_wal with
+                "Htermc Hterml Hlsnc Hlog Hwalfile HinvO") as %Hwal.
+    { apply Hnidme. }
+    (* Read the WAL file. *)
+    wp_apply (wp_FileReadOp with "Hfile").
+    iIntros (err p len) "[Hfile HdataP]".
+    (* Close the core invariant. *)
+    iMod ("HinvC" with "HinvO") as "_".
+    iModIntro.
+    iDestruct ("HinvnodeC" with "[Hwalfile Hfile]") as "HinvfileO".
+    { iFrame "∗ # %". }
+    iMod ("HinvfileC" with "HinvfileO") as "_".
+    iModIntro.
+    destruct err; wp_pures.
+    { wp_apply wp_Exit. iIntros "[]". }
+    iDestruct "HdataP" as "[%Hlen HdataP]".
+    set dataP := Slice.mk p len len.
+    iDestruct (pointsto_vals_own_slice_small_byte dataP with "HdataP") as "Hdata".
+    { done. }
+    { done. }
+    wp_apply wp_ref_to.
+    { apply (slice_val_ty dataP). }
+    iIntros (dataPP) "HdataPP".
+    wp_pures.
+
     (*@     for 0 < uint64(len(data)) {                                         @*)
     (*@         kind, data = marshal.ReadInt(data)                              @*)
     (*@                                                                         @*)
-    (*@         if kind == CMD_EXTEND {                                         @*)
-    (*@             ents, data = util.DecodeStrings(data)                       @*)
-    (*@                                                                         @*)
-    (*@             log = append(log, ents...)                                  @*)
-    (*@         } else if kind == CMD_APPEND {                                  @*)
-    (*@             ents = make([]string, 1)                                    @*)
-    (*@             var ent string                                              @*)
-    (*@             ent, data = util.DecodeString(data)                         @*)
-    (*@                                                                         @*)
-    (*@             log = append(log, ent)                                      @*)
-    (*@         } else if kind == CMD_PREPARE {                                 @*)
-    (*@             term, data = marshal.ReadInt(data)                          @*)
-    (*@                                                                         @*)
-    (*@             termc = term                                                @*)
-    (*@         } else if kind == CMD_ADVANCE {                                 @*)
-    (*@             term, data = marshal.ReadInt(data)                          @*)
-    (*@             lsn, data = marshal.ReadInt(data)                           @*)
-    (*@             ents, data = util.DecodeStrings(data)                       @*)
-    (*@                                                                         @*)
-    (*@             terml = term                                                @*)
-    (*@             // Prove safety of this triming operation using well-formedness of @*)
-    (*@             // the write-ahead log. See [execute_paxos_advance] in recovery.v. @*)
-    (*@             log = log[: lsn]                                            @*)
-    (*@             log = append(log, ents...)                                  @*)
-    (*@         } else if kind == CMD_ACCEPT {                                  @*)
-    (*@             lsn, data = marshal.ReadInt(data)                           @*)
-    (*@             ents, data = util.DecodeStrings(data)                       @*)
-    (*@                                                                         @*)
-    (*@             // Prove safety of this triming operation using well-formedness of @*)
-    (*@             // the write-ahead log. See [execute_paxos_accept] in recovery.v. @*)
-    (*@             log = log[: lsn]                                            @*)
-    (*@             log = append(log, ents...)                                  @*)
-    (*@         } else if kind == CMD_EXPAND {                                  @*)
-    (*@             lsn, data = marshal.ReadInt(data)                           @*)
-    (*@                                                                         @*)
-    (*@             lsnc = lsn                                                  @*)
-    (*@         }                                                               @*)
-    (*@     }                                                                   @*)
-    (*@                                                                         @*)
+    set P := (λ cont : bool,
+                ∃ (q : Slice.t) (applied remaining : list w8) (wala walr : list pxcmd)
+                  (termca termla lsnca : u64) (logaP : Slice.t) (loga : list byte_string),
+                  let pxst := PaxosState (uint.nat termca) (uint.nat termla) (uint.nat lsnca) loga in
+                  "HdataPP" ∷ dataPP ↦[slice.T byteT] q ∗
+                  "Hdata"   ∷ own_slice_small q byteT (DfracOwn 1) remaining ∗
+                  "HtermcP" ∷ termcP ↦[uint64T] #termca ∗
+                  "HtermlP" ∷ termlP ↦[uint64T] #termla ∗
+                  "HlsncP"  ∷ lsncP ↦[uint64T] #lsnca ∗
+                  "HlogPP"  ∷ logPP ↦[slice.T stringT] (to_val logaP) ∗
+                  "HlogP"   ∷ own_slice logaP stringT (DfracOwn 1) loga ∗
+                  "%Hwalar" ∷ ⌜wal = wala ++ walr⌝ ∗
+                  "%Hwala"  ∷ ⌜encode_paxos_cmds wala = applied⌝ ∗
+                  "%Hwalr"  ∷ ⌜encode_paxos_cmds walr = remaining⌝ ∗
+                  "%Hexec"  ∷ ⌜execute_paxos_cmds wala = pxst⌝ ∗
+                  "%Hcont"  ∷ ⌜if cont then True else length remaining = O⌝)%I.
+    wp_apply (wp_forBreak_cond P with
+               "[] [HdataPP Hdata $HtermcP $HtermlP $HlsncP $HlogPP $HlogP]");
+      last first; first 1 last.
+    { iExists dataP.
+      iFrame.
+      iPureIntro. simpl.
+      by exists [], [], wal.
+    }
+    { clear Φ.
+      iIntros (Φ) "!> HP HΦ".
+      iNamed "HP".
+      wp_load.
+      wp_apply wp_slice_len.
+      wp_pures.
+      iDestruct (own_slice_small_sz with "Hdata") as %Hlenr.
+      case_bool_decide as Hbound; wp_pures; last first.
+      { iApply "HΦ".
+        iFrame "∗ %".
+        iPureIntro.
+        clear -Hbound Hlenr. word.
+      }
+      assert (Hrem : length remaining ≠ O).
+      { clear -Hbound Hlenr. word. }
+      destruct walr as [| cmd walr'] eqn:Hwalreq.
+      { apply length_not_nil_inv in Hrem.
+        by rewrite /encode_paxos_cmds serialize_nil in Hwalr.
+      }
+      wp_load.
+      assert (Hvdcmd : valid_wal_entry cmd).
+      { rewrite Forall_forall in Hvdwal.
+        apply Hvdwal.
+        rewrite Hwalar.
+        set_solver.
+      }
+      rewrite -Hwalr.
+      rewrite /encode_paxos_cmds serialize_cons.
+      destruct cmd eqn:Hcmd; rewrite {1}/encode_paxos_cmd /encode_paxos_extend -app_assoc.
+      { (* Case: Extend. *)
+
+        (*@         if kind == CMD_EXTEND {                                         @*)
+        (*@             ents, bs1 := util.DecodeStrings(bs)                         @*)
+        (*@             data = bs1                                                  @*)
+        (*@             // Apply extend.                                            @*)
+        (*@             log = append(log, ents...)                                  @*)
+        (*@                                                                         @*)
+        wp_apply (wp_ReadInt with "Hdata").
+        iIntros (q') "Hdata".
+        wp_apply (wp_DecodeStrings with "Hdata").
+        iIntros (s bs1) "[Hents Hdata]".
+        wp_store.
+        wp_load.
+        iDestruct (own_slice_to_small with "Hents") as "Hents".
+        wp_apply (wp_SliceAppendSlice with "[$HlogP $Hents]"); first done.
+        iIntros (logaP') "[HlogP Hents]".
+        wp_store.
+        iApply "HΦ".
+        iFrame "HlogPP ∗".
+        iPureIntro. simpl.
+        exists (applied ++ encode_paxos_cmd cmd), (wala ++ [cmd]), walr'.
+        split.
+        { by rewrite Hwalar -app_assoc Hcmd. }
+        split.
+        { by rewrite encode_paxos_cmds_snoc Hwala. }
+        split; first done.
+        split.
+        { by rewrite execute_paxos_cmds_snoc Hexec Hcmd /=. }
+        done.
+      }
+      { (* Case: Append. *)
+
+        (*@         } else if kind == CMD_APPEND {                                  @*)
+        (*@             ent, bs1 := util.DecodeString(bs)                           @*)
+        (*@             data = bs1                                                  @*)
+        (*@             // Apply append.                                            @*)
+        (*@             log = append(log, ent)                                      @*)
+        (*@                                                                         @*)
+        wp_apply (wp_ReadInt with "Hdata").
+        iIntros (q') "Hdata".
+        wp_apply (wp_DecodeString with "Hdata").
+        iIntros (bs1) "Hdata".
+        wp_store.
+        wp_load.
+        wp_apply (wp_SliceAppend with "[$HlogP]").
+        iIntros (logaP') "HlogP".
+        wp_store.
+        iApply "HΦ".
+        iFrame "HlogPP ∗".
+        iPureIntro. simpl.
+        exists (applied ++ encode_paxos_cmd cmd), (wala ++ [cmd]), walr'.
+        split.
+        { by rewrite Hwalar -app_assoc Hcmd. }
+        split.
+        { by rewrite encode_paxos_cmds_snoc Hwala. }
+        split; first done.
+        split.
+        { by rewrite execute_paxos_cmds_snoc Hexec Hcmd /=. }
+        done.
+      }
+      { (* Case: Prepare. *)
+
+        (*@         } else if kind == CMD_PREPARE {                                 @*)
+        (*@             term, bs1 := marshal.ReadInt(bs)                            @*)
+        (*@             data = bs1                                                  @*)
+        (*@             // Apply prepare.                                           @*)
+        (*@             termc = term                                                @*)
+        (*@                                                                         @*)
+        wp_apply (wp_ReadInt with "Hdata").
+        iIntros (q') "Hdata".
+        wp_apply (wp_ReadInt with "Hdata").
+        iIntros (bs1) "Hdata".
+        do 2 wp_store.
+        iApply "HΦ".
+        iFrame "HlogPP ∗".
+        iPureIntro. simpl.
+        exists (applied ++ encode_paxos_cmd cmd), (wala ++ [cmd]), walr'.
+        split.
+        { by rewrite Hwalar -app_assoc Hcmd. }
+        split.
+        { by rewrite encode_paxos_cmds_snoc Hwala. }
+        split; first done.
+        split.
+        { (* Prove [term] fit into u64. *)
+          simpl in Hvdcmd.
+          rewrite execute_paxos_cmds_snoc Hexec Hcmd /=.
+          f_equal.
+          clear -Hvdcmd. word.
+        }
+        done.
+      }
+      { (* Case: Advance. *)
+
+        (*@         } else if kind == CMD_ADVANCE {                                 @*)
+        (*@             term, bs1 := marshal.ReadInt(bs)                            @*)
+        (*@             lsn, bs2 := marshal.ReadInt(bs1)                            @*)
+        (*@             ents, bs3 := util.DecodeStrings(bs2)                        @*)
+        (*@             data = bs3                                                  @*)
+        (*@             // Apply advance.                                           @*)
+        (*@             terml = term                                                @*)
+        (*@             // Prove safety of this triming operation using well-formedness of @*)
+        (*@             // the write-ahead log. See [execute_paxos_advance] in recovery.v. @*)
+        (*@             log = log[: lsn]                                            @*)
+        (*@             log = append(log, ents...)                                  @*)
+        (*@                                                                         @*)
+        wp_apply (wp_ReadInt with "Hdata").
+        iIntros (q') "Hdata".
+        wp_apply (wp_ReadInt with "Hdata").
+        iIntros (bs1) "Hdata".
+        wp_apply (wp_ReadInt with "Hdata").
+        iIntros (bs2) "Hdata".
+        wp_apply (wp_DecodeStrings with "Hdata").
+        iIntros (s bs3) "[Hents Hdata]".
+        do 2 wp_store.
+        wp_load.
+        assert (Hsafetrim : (lsn ≤ length loga)%nat).
+        { unshelve epose proof (execute_paxos_cmds_prefix_not_stuck (wala ++ [cmd]) wal _ _) as Hns.
+          { rewrite Hwalar Hcmd.
+            apply prefix_app, prefix_cons, prefix_nil.
+          }
+          { by rewrite Hwal. }
+          rewrite execute_paxos_cmds_snoc Hexec Hcmd in Hns.
+          rewrite /execute_paxos_cmds /execute_paxos_cmd in Hns.
+          by apply execute_paxos_advance_safely_trimmed in Hns.
+        }
+        wp_apply (wp_SliceTake_full with "HlogP").
+        { clear -Hsafetrim. word. }
+        iIntros "HlogP".
+        wp_store.
+        wp_load.
+        iDestruct (own_slice_to_small with "Hents") as "Hents".
+        wp_apply (wp_SliceAppendSlice with "[$HlogP $Hents]"); first done.
+        iIntros (logaP') "[HlogP Hents]".
+        wp_store.
+        iApply "HΦ".
+        iFrame "HlogPP ∗".
+        iPureIntro. simpl.
+        exists (applied ++ encode_paxos_cmd cmd), (wala ++ [cmd]), walr'.
+        split.
+        { by rewrite Hwalar -app_assoc Hcmd. }
+        split.
+        { by rewrite encode_paxos_cmds_snoc Hwala. }
+        split; first done.
+        split.
+        { (* Prove [term] and [lsn] fit into u64. *)
+          simpl in Hvdcmd.
+          rewrite execute_paxos_cmds_snoc Hexec Hcmd /=.
+          case_decide; last word.
+          replace (uint.nat (W64 lsn)) with lsn; last first.
+          { clear -Hvdcmd. word. }
+          f_equal.
+          clear -Hvdcmd. word.
+        }
+        done.
+      }
+      { (* Case: Accept. *)
+
+        (*@         } else if kind == CMD_ACCEPT {                                  @*)
+        (*@             lsn, bs1 := marshal.ReadInt(bs)                             @*)
+        (*@             ents, bs2 := util.DecodeStrings(bs1)                        @*)
+        (*@             data = bs2                                                  @*)
+        (*@             // Apply accept.                                            @*)
+        (*@             // Prove safety of this triming operation using well-formedness of @*)
+        (*@             // the write-ahead log. See [execute_paxos_accept] in recovery.v. @*)
+        (*@             log = log[: lsn]                                            @*)
+        (*@             log = append(log, ents...)                                  @*)
+        (*@                                                                         @*)
+        wp_apply (wp_ReadInt with "Hdata").
+        iIntros (q') "Hdata".
+        wp_apply (wp_ReadInt with "Hdata").
+        iIntros (bs1) "Hdata".
+        wp_apply (wp_DecodeStrings with "Hdata").
+        iIntros (s bs3) "[Hents Hdata]".
+        wp_store.
+        wp_load.
+        assert (Hsafetrim : (lsn ≤ length loga)%nat).
+        { unshelve epose proof (execute_paxos_cmds_prefix_not_stuck (wala ++ [cmd]) wal _ _) as Hns.
+          { rewrite Hwalar Hcmd.
+            apply prefix_app, prefix_cons, prefix_nil.
+          }
+          { by rewrite Hwal. }
+          rewrite execute_paxos_cmds_snoc Hexec Hcmd in Hns.
+          rewrite /execute_paxos_cmds /execute_paxos_cmd in Hns.
+          by apply execute_paxos_accept_safely_trimmed in Hns.
+        }
+        wp_apply (wp_SliceTake_full with "HlogP").
+        { clear -Hsafetrim. word. }
+        iIntros "HlogP".
+        wp_store.
+        wp_load.
+        iDestruct (own_slice_to_small with "Hents") as "Hents".
+        wp_apply (wp_SliceAppendSlice with "[$HlogP $Hents]"); first done.
+        iIntros (logaP') "[HlogP Hents]".
+        wp_store.
+        iApply "HΦ".
+        iFrame "HlogPP ∗".
+        iPureIntro. simpl.
+        exists (applied ++ encode_paxos_cmd cmd), (wala ++ [cmd]), walr'.
+        split.
+        { by rewrite Hwalar -app_assoc Hcmd. }
+        split.
+        { by rewrite encode_paxos_cmds_snoc Hwala. }
+        split; first done.
+        split.
+        { (* Prove [lsn] fit into u64. *)
+          simpl in Hvdcmd.
+          rewrite execute_paxos_cmds_snoc Hexec Hcmd /=.
+          case_decide; last word.
+          replace (uint.nat (W64 lsn)) with lsn; last first.
+          { clear -Hvdcmd. word. }
+          done.
+        }
+        done.
+      }
+      { (* Case: Expand. *)
+
+        (*@         } else if kind == CMD_EXPAND {                                  @*)
+        (*@             lsn, bs1 := marshal.ReadInt(bs)                             @*)
+        (*@             data = bs1                                                  @*)
+        (*@             // Apply expand.                                            @*)
+        (*@             lsnc = lsn                                                  @*)
+        (*@         }                                                               @*)
+        (*@                                                                         @*)
+        wp_apply (wp_ReadInt with "Hdata").
+        iIntros (q') "Hdata".
+        wp_apply (wp_ReadInt with "Hdata").
+        iIntros (bs1) "Hdata".
+        do 2 wp_store.
+        iApply "HΦ".
+        iFrame "HlogPP ∗".
+        iPureIntro. simpl.
+        exists (applied ++ encode_paxos_cmd cmd), (wala ++ [cmd]), walr'.
+        split.
+        { by rewrite Hwalar -app_assoc Hcmd. }
+        split.
+        { by rewrite encode_paxos_cmds_snoc Hwala. }
+        split; first done.
+        split.
+        { (* Prove [lsn] fit into u64. *)
+          simpl in Hvdcmd.
+          rewrite execute_paxos_cmds_snoc Hexec Hcmd /=.
+          f_equal.
+          clear -Hvdcmd. word.
+        }
+        done.
+      }
+    }
+
     (*@     return termc, terml, lsnc, log                                      @*)
     (*@ }                                                                       @*)
-  Admitted.
+    iNamed 1.
+    do 4 wp_load.
+    wp_pures.
+    assert (walr = []) as ->.
+    { apply encode_paxos_cmds_nil_inv, nil_length_inv.
+      by rewrite Hwalr.
+    }
+    rewrite app_nil_r in Hwalar. subst wala.
+    rewrite Hwal in Hexec.
+    inv Hexec.
+    rewrite -(uint_nat_u64_inj _ _ H0).
+    rewrite -(uint_nat_u64_inj _ _ H1).
+    rewrite -(uint_nat_u64_inj _ _ H2).
+    iApply ("HΦ" $! logaP).
+    by iFrame.
+  Qed.
 
 End resume.
